stuck on id-substitution

formalization/typedjs.v
@@ -11,6 +11,246 @@ Inductive typ : Set :=
 
 Axiom typ_union_symm : forall t1 t2, typ_union t1 t2 = typ_union t2 t1.
 
+Inductive string : Set :=
+  | str_number : string
+  | str_boolean : string
+  | str_function : string
+  | str_string : string
+  | str_other_string : string.
+
+Inductive split : Set :=
+  | split_bvar : nat -> RTS -> RTS -> split
+  | no_split : split.
+
+Inductive exp : Set :=
+  | e_bvar : RTS -> nat -> exp
+  | e_fvar : RTS -> atom -> exp
+  | e_equal : exp -> exp -> exp
+  | e_typeof : exp -> exp
+  | e_if : split -> exp -> exp -> exp -> exp
+  | e_app : exp -> exp -> exp
+  (* Unlike the POPL tutorial, we need typ on e_abs for lc *)
+  | e_abs : typ -> exp -> exp
+  | e_num : nat -> exp
+  | e_str : string -> exp
+  | e_bool : bool -> exp.
+
+
+(** Substitute z for u in e.  Assume that u is locally closed. *)
+Fixpoint subst (z : atom) (u : exp) (e : exp) {struct e} : exp :=
+  match e with
+  | e_bvar r n => e_bvar r n
+  | e_fvar r x => if x == z then u else e_fvar r x
+  | e_equal e1 e2 => e_equal (subst z u e1) (subst z u e2)
+  | e_typeof e1 => e_typeof (subst z u e1)
+  | e_if s e1 e2 e3 => e_if s (subst z u e1) (subst z u e2) (subst z u e3)
+  | e_app e1 e2 => e_app (subst z u e1) (subst z u e2)
+  | e_abs t e1 => e_abs t (subst z u e1)
+  | e_num n => e_num n
+  | e_str s => e_str s
+  | e_bool b => e_bool b
+  end.
+
+Fixpoint fv (e : exp) {struct e} : atoms :=
+  match e with
+  | e_bvar r i => {}
+  | e_fvar r x => singleton x
+  | e_equal e1 e2 => (fv e1) `union` (fv e2)
+  | e_typeof e1 => fv e1
+  | e_if s e1 e2 e3 => (fv e1) `union` (fv e2) `union` (fv e3)
+  | e_app e1 e2 => (fv e1) `union` (fv e2)
+  | e_abs t e1 => fv e1
+  | e_num _ => {}
+  | e_str _ => {}
+  | e_bool _ => {}
+  end.
+
+Lemma subst_fresh : forall (x : atom) e u,
+  x `notin` fv e -> subst x u e = e.
+Proof.
+  intros x e u.
+  intros H.
+  induction e; try (simpl; reflexivity).
+  (* e_fvar *)
+  simpl. destruct (a == x). subst a. simpl in H. destruct H. fsetdec. 
+                            reflexivity.
+  (* e_equal *)
+  simpl. simpl in H.
+  assert (x `notin` fv e1). fsetdec. apply IHe1 in H0.
+  assert (x `notin` fv e2). fsetdec. apply IHe2 in H1.
+  rewrite -> H0. rewrite -> H1. reflexivity.
+  (* e_typeof *)
+  simpl. simpl in H. apply IHe in H. rewrite -> H. reflexivity.
+  (* e_if *)
+  simpl. simpl in H.
+  assert (x `notin` fv e1). fsetdec. apply IHe1 in H0.
+  assert (x `notin` fv e2). fsetdec. apply IHe2 in H1.
+  assert (x `notin` fv e3). fsetdec. apply IHe3 in H2.
+  rewrite -> H0. rewrite -> H1. rewrite -> H2. reflexivity.
+  (* e_app *)
+  simpl. simpl in H.
+  assert (x `notin` fv e1). fsetdec. apply IHe1 in H0.
+  assert (x `notin` fv e2). fsetdec. apply IHe2 in H1.
+  rewrite -> H0. rewrite -> H1. reflexivity.
+  (* e_abs *)
+  simpl. simpl in H. apply IHe in H. rewrite -> H. reflexivity.
+Qed.
+
+
+(** Opening *)
+
+Definition typeof (e : exp) : option RT:=
+  match e with
+  | e_bool _ => Some rt_boolean
+  | e_num _ => Some rt_number
+  | _ => None
+  end.
+
+
+Fixpoint open_rec (k : nat) (u : exp) (e : exp) {struct e} : exp :=
+  match e with
+  | e_bvar r i => 
+      if k === i 
+        then match u with
+             | e_fvar _ x => e_fvar r x
+             | _ => u
+             end
+        else e_bvar r i
+  | e_fvar r x => e_fvar r x
+  | e_equal e1 e2 => e_equal (open_rec k u e1) (open_rec k u e2)
+  | e_typeof e1 => e_typeof (open_rec k u e1)
+  | e_if s e1 e2 e3 => 
+      match s with
+      | no_split => e_if no_split (open_rec k u e1) (open_rec k u e2) (open_rec k u e3)
+      | split_bvar k' r1 r2 => if k' === k then
+          match typeof u with
+          | Some r => match rts.mem r r1, rts.mem r r2 with
+                      | true, false => open_rec k u e2
+                      | false, true => open_rec k u e3
+                      | _, _ => e_if no_split (open_rec k u e1) (open_rec k u e2) (open_rec k u e3)
+                      end
+          | None => e_if no_split (open_rec k u e1) (open_rec k u e2) (open_rec k u e3) 
+          end else
+          e_if s (open_rec k u e1) (open_rec k u e2) (open_rec k u e3)
+      end
+  | e_app e1 e2 => e_app (open_rec k u e1) (open_rec k u e2)
+  | e_abs t e1 => e_abs t (open_rec (S k) u e1)
+  | e_num n => e_num n
+  | e_str s => e_str s
+  | e_bool b => e_bool b
+  end.
+
+Definition open e u := open_rec 0 u e.
+
+Hint Unfold open.
+
+Fixpoint runtime (t : typ) { struct t } : rts.t:=
+  match t with
+  | typ_integer =>  rts.singleton rt_number
+  | typ_string => rts.singleton rt_string
+  | typ_boolean => rts.singleton rt_boolean
+  | typ_arrow _ _ => rts.singleton rt_function
+  | typ_union t1 t2 => rts.union (runtime t1) (runtime t2)
+  end.
+
+
+Inductive lc : exp -> Prop :=
+  (* e_bvar is not locally closed.  They get substituted out when
+     opening in lc_abs *)
+  | lc_fvar : forall x r, lc (e_fvar r x)
+  | lc_equal : forall e1 e2, lc e1 -> lc e2 -> lc (e_equal e1 e2)
+  | lc_typeof : forall e1, lc e1 -> lc (e_typeof e1)
+  | lc_if : forall s e1 e2 e3, lc e1 -> lc e2 -> lc e3 -> lc (e_if s e1 e2 e3)
+  | lc_app : forall e1 e2, lc e1 -> lc e2 -> lc (e_app e1 e2)
+  | lc_abs : forall L t e1, 
+      (forall x, x `notin` L -> lc (open e1 (e_fvar (runtime t) x))) ->
+      lc (e_abs t e1)
+  | lc_num : forall n, lc (e_num n)
+  | lc_str : forall s, lc (e_str s)
+  | lc_bool : forall b, lc (e_bool b).
+
+Hint Constructors lc.
+
+
+Inductive value : exp -> Prop :=
+  | value_num : forall n, value (e_num n)
+  | value_str : forall s, value (e_str s)
+  | value_bool : forall b, value (e_bool b)
+  | value_abs : forall t e, lc (e_abs t e) -> value (e_abs t e).
+
+Inductive eval : exp -> exp -> Prop :=
+  | eval_beta : forall t e1 e2,
+      lc (e_abs t e1) -> value e2 ->
+      eval (e_app (e_abs t e1) e2) (open e1 e2)
+  | eval_equal_true : forall v1 v2, value v1 -> value v2 ->
+      v1 = v2 -> eval (e_equal v1 v2) (e_bool true)
+  | eval_equal_false : forall v1 v2, value v1 -> value v2 ->
+      v1 <> v2 -> eval (e_equal v1 v2) (e_bool false)
+  | eval_typeof_str : forall s, 
+      eval (e_typeof (e_str s)) (e_str str_string)
+  | eval_typeof_bool : forall b,
+      eval (e_typeof (e_bool b)) (e_str str_boolean)
+  | eval_typeof_num : forall n,
+      eval (e_typeof (e_num n)) (e_str str_number)
+  | eval_typeof_abs : forall t e1, lc (e_abs t e1) ->
+      eval (e_typeof (e_abs t e1)) (e_str str_function)
+  | e_if_true : forall e1 e2, lc e1 -> lc e2 ->
+      eval (e_if no_split (e_bool true) e1 e2) e1
+  | e_if_false : forall e1 e2, lc e1 -> lc e2 ->
+      eval (e_if no_split (e_bool false) e1 e2) e2
+  | cxt_equal_1 : forall e1 e1' e2, lc e2 -> eval e1 e1' ->
+      eval (e_equal e1 e2) (e_equal e1' e2)
+  | cxt_equal_2 : forall e1 e2 e2', value e1 -> eval e2 e2' ->
+      eval (e_equal e1 e2) (e_equal e1 e2')
+  | cxt_typeof : forall e e', eval e e' ->
+      eval (e_typeof e) (e_typeof e')
+  | cxt_if : forall s e1 e1' e2 e3, eval e1 e1' -> lc e2 -> lc e3 ->
+      eval (e_if s e1 e2 e3) (e_if s e1' e2 e3)
+  | cxt_app_1 : forall e1 e1' e2, lc e2 ->
+      eval e1 e1' ->
+      eval (e_app e1 e2) (e_app e1' e2)
+  | cxt_app_2 : forall e1 e2 e2',
+      value e1 ->
+      eval e2 e2' ->
+      eval (e_app e1 e2) (e_app e1 e2').
+
+Inductive eval_multi : exp -> exp -> Prop :=
+  | m_trans : forall e1 e2 e3, eval e1 e2 -> eval_multi e2 e3 -> eval_multi e1 e3
+  | m_step : forall e1 e2, eval e1 e2 -> eval_multi e1 e2.
+
+Hint Constructors value eval eval_multi.
+
+Ltac gather_atoms :=
+  let A := gather_atoms_with (fun x : atoms => x) in
+  let B := gather_atoms_with (fun x : atom => singleton x) in
+  let C := gather_atoms_with (fun x : list (atom * typ) => dom x) in
+  let D := gather_atoms_with (fun x : exp => fv x) in
+  constr:(A `union` B `union` C `union` D).
+
+Tactic Notation
+      "pick" "fresh" ident(atom_name) "and" "apply" constr(lemma) :=
+  let L := gather_atoms in
+  pick fresh atom_name excluding L and apply lemma.
+
+Notation env := (list (atom * typ)).
+
+Fixpoint static (rt : rts.t) (t : typ) { struct t } : option typ := 
+  match t with
+  | typ_integer => if rts.mem rt_number rt then (Some typ_integer) else None
+  | typ_string => if rts.mem rt_string rt then (Some typ_string) else None
+  | typ_boolean => if rts.mem rt_boolean rt then (Some typ_boolean) else None
+  | typ_arrow _ _ => if rts.mem rt_function rt then (Some t) else None
+  | typ_union t1 t2 => 
+      match static rt t1, static rt t2 with
+      | None, None => None
+      | Some t1', Some t2' => Some (typ_union t1' t2')
+      | Some t1', None => Some t1'
+      | None, Some t2' => Some t2'
+      end
+  end.
+
+
+
 Inductive subtype : typ -> typ -> Prop :=
   | subtype_invariant : forall (t : typ), subtype t t
   | subtype_trans : forall (s t u : typ), 
@@ -22,6 +262,275 @@ Inductive subtype : typ -> typ -> Prop :=
       subtype s1 t /\ subtype s2 t -> subtype (typ_union s1 s2) t
   | subtype_unionR : forall (s t1 t2 : typ),
       subtype s t1 \/ subtype s t2 -> subtype s (typ_union t1 t2).
+
+Inductive typing : env -> exp -> typ -> Prop :=
+  | typing_var : forall E (v : atom) R T T',
+      ok E -> 
+      binds v T E ->
+      static R T = Some T' ->
+      typing E (e_fvar R v) T'
+  | typing_abs : forall L E e T1 T2,
+      (forall (v : atom), v `notin` L ->
+         typing ((v, T1) :: E) (open e (e_fvar (runtime T1) v)) T2) ->
+      typing E (e_abs T1 e) (typ_arrow T1 T2)
+  | typing_equal : forall E e1 e2 T,
+      typing E e1 T ->
+      typing E e2 T ->
+      typing E (e_equal e1 e2) typ_boolean
+  | typing_typeof : forall E e1 T,
+      typing E e1 T ->
+      typing E (e_typeof e1) typ_string
+  | typing_if : forall E e1 e2 e3 T s,
+      typing E e1 typ_boolean ->
+      typing E e2 T ->
+      typing E e3 T ->
+      typing E (e_if s e1 e2 e3) T
+  | typing_app : forall E e1 e2 T1 T2,
+      typing E e1 (typ_arrow T1 T2) ->
+      typing E e2 T1 ->
+      typing E (e_app e1 e2) T2
+  | typing_num : forall E n, typing E (e_num n) typ_integer
+  | typing_str : forall E s, typing E (e_str s) typ_string
+  | typing_bool : forall E b, typing E (e_bool b) typ_boolean.
+
+Hint Constructors typing.
+
+Definition Number := rts.singleton rt_number.
+Definition String := rts.singleton rt_string.
+
+Hint Unfold Number String.
+
+Example eg_typing_1 : 
+  typing nil (e_num 9000) typ_integer.
+Proof.
+  apply typing_num.
+Qed.
+
+Example eg_typing_2 :
+  typing nil (e_abs typ_integer (e_bvar (rts.singleton rt_number) 0))
+             (typ_arrow typ_integer typ_integer).
+Proof.
+  pick fresh v and apply typing_abs.
+  unfold open. simpl.
+  apply typing_var with (T := typ_integer).
+  auto. auto. auto.
+Qed.
+
+Lemma strong_weakening : forall E F G e T,
+  typing (G ++ E) e T ->
+  ok (G ++ F ++ E) ->
+  typing (G ++ F ++ E) e T.
+Proof.
+  intros E F G e T H.
+  remember (G ++ E) as E'.
+  generalize dependent G.
+  induction H; intros G Eq Ok; subst.
+  (* e_fvar *)
+  apply typing_var with (T := T). exact Ok. 
+  apply binds_weaken with (F := F) in H0. exact H0. exact Ok. exact H1.
+  (* e_abs *)
+  pick fresh v and apply typing_abs.
+  apply H0 with (G0 := (v, T1) :: G).
+  fsetdec.
+  rewrite -> cons_concat_assoc. reflexivity.
+  rewrite -> cons_concat_assoc. auto.
+  (* e_equal *)
+  apply typing_equal with (T := T).
+  apply IHtyping1 with (G0 := G); auto.
+  apply IHtyping2 with (G0 := G); auto.
+  (* e_type *)
+  apply typing_typeof with (T := T).
+  apply IHtyping with (G0 := G); auto.
+  apply typing_if with (T := T).
+  apply IHtyping1 with (G0 := G); auto.
+  apply IHtyping2 with (G0 := G); auto.
+  apply IHtyping3 with (G0 := G); auto.
+  (* e_app *)
+  apply typing_app with (T1 := T1).
+  apply IHtyping1; auto.
+  apply IHtyping2; auto.
+  (* constants *)
+  apply typing_num.
+  apply typing_str.
+  apply typing_bool.
+Qed.
+
+Lemma weakening : forall E F e T,
+    typing E e T ->
+    ok (F ++ E) ->
+    typing (F ++ E) e T.
+Proof.
+  intros E F e T H J.
+  rewrite <- (nil_concat _ (F ++ E)).
+  apply strong_weakening; auto.
+Qed.
+
+Lemma typing_regular_lc : forall E e T,
+  typing E e T -> lc e.
+Proof.
+  intros E e T H. induction H; eauto.
+Qed.
+
+Lemma substitution_var : forall E F u S T T' w v R,
+  binds v T' (F ++ (w, S) :: E) ->
+  ok (F ++ (w, S) :: E) ->
+  Some T = static R T' ->
+  typing E u S ->
+  typing (F ++ E) (subst w u (e_fvar R v)) T.
+Proof.
+  intros E F u S T T' w v R Binds Ok Static H.
+  simpl.
+  destruct (v == w).
+  Focus 2.
+  (* v <> w, nothing to do *)
+  apply typing_var with (T := T').
+  apply ok_remove_mid_cons with (x := w) (a := S). exact Ok.
+  apply binds_remove_mid with (y := w) (b := S). simpl. exact Binds. exact n.
+  rewrite -> Static. reflexivity.
+  (* v = w, substitution happens *)
+  assert (T = S) as HypTeqS.
+    rewrite -> e in Binds.
+    apply binds_mid_eq with (F := F) (z := w) (E := E). simpl. exact Binds.
+
+
+Example eg_typing_3 :
+  typing nil
+    (e_abs (e_if (split_bvar 0 Number String) 
+                 (e_equal (e_typeof (e_bvar (rts.union Number String) 0))
+                          (e_str str_number))
+                 (e_bvar Number 0)
+                 (e_num 42)))
+    (typ_arrow (typ_union typ_integer typ_string) typ_integer).
+Proof.
+  pick fresh v and apply typing_abs.
+  unfold open. simpl.
+  apply typing_if.
+  apply typing_equal with (T := typ_string).
+  apply typing_typeof with (T := typ_union typ_integer typ_string).
+  apply typing_var with (T := (typ_union typ_integer typ_string)). auto. auto. auto.
+  apply typing_str.
+  apply typing_var with (T := typ_union typ_integer typ_string). auto. auto. auto.
+  apply typing_num.
+Qed.
+
+Example eg_eval_if : eval (e_if no_split (e_bool true) (e_num 50) (e_num 20)) 
+                          (e_num 50).
+  auto.
+Qed.
+
+
+
+Example eg_eval_app_if :
+  eval (e_app (e_abs (e_if no_split (e_bvar (rts.singleton rt_boolean) 0) (e_num 42) (e_num 90))) (e_bool true))
+       (e_if no_split (e_bool true) (e_num 42) (e_num 90)).
+Proof.
+  assert (open (e_if no_split (e_bvar (rts.singleton rt_boolean) 0) (e_num 42) (e_num 90)) (e_bool true) =
+               (e_if no_split (e_bool true) (e_num 42) (e_num 90))).
+    auto.
+  rewrite <- H. 
+  apply eval_beta.
+    (* prove local closure *)
+    apply lc_abs with (L := {}).
+      intros. unfold open. simpl. auto.
+    (* prove that (e_bool true) is a value *)
+    auto.
+Qed.
+
+Example eg_eval_multi_app_if :
+    eval_multi (e_app (e_abs (e_if no_split (e_bvar (rts.singleton rt_boolean) 0) (e_num 42) (e_num 90))) (e_bool true))
+         (e_num 42).
+Proof.
+  apply m_trans with (e2 := e_if no_split (e_bool true) (e_num 42) (e_num 90)).
+    apply eg_eval_app_if.
+  auto.
+Qed.
+  
+
+(*
+  (lambda (x) // x : typ_union int string
+    (if (equal? (typeof x) "string")
+      (string-append x "hello")
+      (+ x 1)))
+
+  (lambda (x) // x : typ_union int string
+    (let ([t (equal? (typeof x) "string")])
+      (if t
+        (string-append x "hello")
+        (+ x 1))))
+
+  (lambda (x)
+    (app (lambda (t)
+      (if t x-string ... x-int))
+     (equal? (typeof x) "string")))
+
+*)
+
+Definition eg0 : exp :=
+   (e_abs (e_app (e_abs (e_if (split_bvar 1 (rts.singleton rt_string) (rts.singleton rt_number))  (e_bvar (rts.singleton rt_boolean) 0)
+                           (e_num 42) 
+                           (e_bvar (rts.singleton rt_number) 1)))
+                 (e_equal 
+                   (e_typeof 
+                     (e_bvar (rts.union (rts.singleton rt_string) (rts.singleton rt_number)) 0))
+                   (e_str str_string)))).
+
+Example eg_eval_ifsplit1 :
+  (eval_multi (e_app eg0 (e_num 9000))
+              (e_num 9000)).
+Proof.
+  unfold eg0.
+  assert (
+    (open (e_app (e_abs (e_if (split_bvar 1 (rts.singleton rt_string) (rts.singleton rt_number))  (e_bvar (rts.singleton rt_boolean) 0)
+                           (e_num 42) 
+                           (e_bvar (rts.singleton rt_number) 1)))
+                 (e_equal 
+                   (e_typeof 
+                     (e_bvar (rts.union (rts.singleton rt_string) (rts.singleton rt_number)) 0))
+                   (e_str str_string)))
+          (e_num 9000)) =
+    (e_app (e_abs (e_num 9000))
+           (e_equal 
+             (e_typeof 
+               (e_num 9000))
+             (e_str str_string))) ).
+    unfold open.  simpl. reflexivity.
+  apply m_trans with (e2 := (e_app (e_abs (e_num 9000))
+           (e_equal 
+             (e_typeof 
+               (e_num 9000))
+             (e_str str_string)))).
+    rewrite <- H. apply eval_beta.
+    apply lc_abs with (L := {}).
+    intros. unfold open. simpl.
+    apply lc_app. apply lc_abs with (L :=  {}).
+    intros. unfold open. simpl. apply lc_if. auto. auto. auto.
+    auto. auto.
+  apply m_step.
+  apply eval_beta with (e1 := e_num 9000) (e2 := 
+           (e_equal 
+             (e_typeof 
+               (e_num 9000))
+             (e_str str_string))).
+  apply lc_abs with (L := {}). intros. unfold open. simpl. apply lc_num.
+  apply H0.
+  
+    simpl. 
+  
+  apply m_trans with (e2 := open (e_app (e_abs (e_if no_split (e_bvar (rts.singleton rt_boolean) 0)
+                           (e_num 42) 
+                           (e_bvar (rts.singleton rt_number) 1))).
+                 (e_equal 
+                   (e_typeof 
+                     (e_bvar (rts.union (rts.singleton rt_string) (rts.singleton rt_number)) 0))
+                   (e_str str_string))) (e_str str_string)).
+    
+    auto.
+  auto.
+
+
+
+
+
 
 Example subtype_eg0 : subtype typ_string (typ_union typ_string typ_boolean).
 Proof.
@@ -85,20 +594,6 @@ Proof with subst.
 
 *)
 
-Fixpoint static (rt : rts.t) (t : typ) { struct t } : option typ := 
-  match t with
-  | typ_integer => if rts.mem rt_number rt then (Some typ_integer) else None
-  | typ_string => if rts.mem rt_string rt then (Some typ_string) else None
-  | typ_boolean => if rts.mem rt_boolean rt then (Some typ_boolean) else None
-  | typ_arrow _ _ => if rts.mem rt_function rt then (Some t) else None
-  | typ_union t1 t2 => 
-      match static rt t1, static rt t2 with
-      | None, None => None
-      | Some t1', Some t2' => Some (typ_union t1' t2')
-      | Some t1', None => Some t1'
-      | None, Some t2' => Some t2'
-      end
-  end.
 
 Theorem type_ordering : forall t r1 r2 t1' t2',
   rts.Subset r1 r2 -> 
@@ -116,14 +611,6 @@ Proof.
   assert (
 
 
-Fixpoint runtime (t : typ) { struct t } : rts.t:=
-  match t with
-  | typ_integer =>  rts.singleton rt_number
-  | typ_string => rts.singleton rt_string
-  | typ_boolean => rts.singleton rt_boolean
-  | typ_arrow _ _ => rts.singleton rt_function
-  | typ_union t1 t2 => rts.union (runtime t1) (runtime t2)
-  end.
 
 
   
